modify ocaml code

compiler/entry/commonCLI.ml
@@ -57,11 +57,12 @@ let after_pass =
   let passes = Arg.enum alts in
   Arg.(value & opt passes Typing & info [ "compile"; "after" ] ~doc)
 
-let parse_and_compile (type reg regx xreg rflag cond asm_op extra_op)
+let parse_and_compile (type reg regx xreg regmask rflag cond asm_op extra_op)
     (module Arch : Arch_full.Arch
       with type reg = reg
        and type regx = regx
        and type xreg = xreg
+       and type regmask = regmask
        and type rflag = rflag
        and type cond = cond
        and type asm_op = asm_op
