compiler/src/coreArchFactory.ml
@@ -15,6 +15,7 @@ let core_arch_x86 ~use_lea ~use_set0 call_conv :
        with type reg = register
         and type regx = register_ext
         and type xreg = xmm_register
+        and type regmask = register_mask
         and type rflag = rflag
         and type cond = condt
         and type asm_op = X86_instr_decl.x86_op
